Code refactor up to TestProps

src/theories/Core/RISCVMachine.v
@@ -3,7 +3,7 @@ Require Import Coq.Lists.List.
 Import List.ListNotations.
 Require Import Bool.
 
-From StackSafety Require Import MachineModule (* PolicyModule *).
+From StackSafety Require Import MachineModule PolicyModule.
 
 Require Import coqutil.Word.Naive.
 Require Import coqutil.Word.Properties.
@@ -33,26 +33,32 @@ Require Import Lia.
 From RecordUpdate Require Import RecordSet.
 Import RecordSetNotations.
 
-(* From QuickChick Require Import QuickChick. *)
+From QuickChick Require Import QuickChick.
 
-Module Type RISCV <: Machine.
+Module RISCV <: Machine.
   Export RiscvMachine.
 
-(* Axiom exception : forall {A}, string -> A. *)
-(* Extract Constant exception => *)
-(*   "(fun l -> *)
-(*    let s = Bytes.create (List.length l) in *)
-(*    let rec copy i = function *)
-(*     | [] -> s *)
-(*     | c :: l -> Bytes.set s i c; copy (i+1) l *)
-(*    in failwith (""Exception: "" ^ Bytes.to_string (copy 0 l)))". *)
+  Axiom exception : forall {A}, string -> A.
+  Extract Constant exception =>
+            "(fun l ->
+            let s = Bytes.create (List.length l) in
+            let rec copy i = function
+                | [] -> s
+                | c :: l -> Bytes.set s i c; copy (i+1) l
+                in failwith (""Exception: "" ^ Bytes.to_string (copy 0 l)))".
 
   Definition Word := MachineInt.
+  Definition Value := Word.
+
+  Definition vtow (v:Value) : Word := v.
+  Definition ztow (z:Z) : Word := z.
+  Definition wtoz (w:Word) : Z := w.
+  
   (* Parameter Word *)
   Definition Addr : Type := Word.
 
-  (* Instance ShowWord : Show word := *)
-  (*   {| show x := show (word.signed x) |}. *)
+   Instance ShowWord : Show word :=
+     {| show x := show (word.signed x) |}.
 
   Definition wlt : Word -> Word -> bool := Z.ltb.
   (*  Parameter wlt : Word -> Word -> bool. *)
@@ -163,10 +169,9 @@ Module Type RISCV <: Machine.
   (* Definition Value : Type := Word. *)
   (* Definition vtow (v : Value) : Word := v. *)
 
-  (* We use a risc-v machine as our machine state and a view as a map from its
-     components to their values. *)
+  (* We use a risc-v machine as our machine state *)
   Definition MachineState := RiscvMachine.
-  (* Definition View := Component -> Value. *)
+
 
   (* Project what we care about from the RiscV state. *)
   Definition proj (m:  MachineState) (k: Element):  Word :=
@@ -188,12 +193,10 @@ Module Type RISCV <: Machine.
       end
     end.
 
-  (* Definition projw := fun m k => vtow (proj m k). *)
-
-  (* Lemma proj_vtow : forall m k, vtow (proj m k) = vtow (projw m k). Proof. intros;auto. Qed. *)
+  Definition projw (m:MachineState) (k:Element) := vtow (proj m k).
 
   (* Maybe name this pullback instead *)
-  Definition jorp (m : MachineState) (k : Element) (v : Word) : MachineState :=
+  Definition jorp (m : MachineState) (k : Element) (v : Value) : MachineState :=
     match k with
     | Mem a =>
       withMem
@@ -203,6 +206,18 @@ Module Type RISCV <: Machine.
       withRegs (map.put (getRegs m) r (word.of_Z v)) m
     | PC =>
       withPc (word.of_Z v) m
+    end.
+
+  Definition jorpw (m : MachineState) (k : Element) (w : Word) : MachineState :=
+    match k with
+    | Mem a =>
+      withMem
+        (unchecked_store_byte_list (word.of_Z a)
+                                   (Z32s_to_bytes [w]) (getMem m)) m
+    | Reg r => 
+      withRegs (map.put (getRegs m) r (word.of_Z w)) m
+    | PC =>
+      withPc (word.of_Z w) m
     end.
   
   Definition getElements (m : MachineState) : list Element :=
@@ -224,10 +239,13 @@ Module Type RISCV <: Machine.
                     (RiscvMachine.getMem m)) in
     pc ++ regs ++ mem.
 
-  Parameter Event : Type.
-
-  Parameter event_eqb : Event -> Event -> bool.
-
+  Definition Event : Type := Register*Word.
+  
+  Definition event_eqb (e1 e2 : Event) : bool :=
+    let '(a1, v1) := e1 in
+    let '(a2, v2) := e1 in
+    andb (weq a1 a2) (weq v1 v2).
+  
   (* Observations are values, or silent (tau) *)
   Inductive Observation : Type := 
   | Out (w:Event)
@@ -252,11 +270,19 @@ Module Type RISCV <: Machine.
   (*   | _, _ => false *)
   (*   end. *)
 
-  (* (* TODO: We don't have information about which parts of memory to monitor for *)
-  (*    changes. On a first approximation, monitor all positions (aligned accesses *)
-  (*    only) outside the code segment (whose limits are here, again for simplicity, *)
-  (*    hardcoded). *) *)
-  Parameter findDiff : MachineState -> MachineState -> option Event.
+  Definition listify1 {A} (m : Zkeyed_map A)
+    : list (Z * A) :=
+    List.rev (map.fold (fun acc z v => (z,v) :: acc) nil m).
+  
+  (* For now we will only monitor registers for changes. We could monitor
+     some memory, but we can't monitor the stack. *)
+  Definition findDiff (mOld mNew : MachineState) : option (Register*Word) :=
+    match find (fun '(reg,_) => negb (weq (proj mOld (Reg reg)) (proj mNew (Reg reg))))
+               (listify1 (getRegs mNew)) with
+    | Some (r, _) =>
+      Some (r, proj mNew (Reg r))
+    | None => None
+    end.
 
   Definition FunID := nat.
   Definition StackID := nat.
@@ -311,7 +337,7 @@ Module Type RISCV <: Machine.
   Definition Operations := list Operation.
 
   Definition CodeMap := Addr -> option Operations.
-
+  
   (* TODO: operations *)
   (* A Machine State can step to a new Machine State plus an Observation. *)
   Definition step (m : MachineState) : MachineState * list Operation * Observation :=
@@ -328,3 +354,223 @@ Module Type RISCV <: Machine.
       end.
 
 End RISCV.
+
+Module RISCVTagged (P : TagPolicy RISCV) <: Machine.
+  Import P.
+  Export RISCV.
+  
+  Definition Word := Word.
+  Definition Value : Type := (Word * Tag).
+  
+  Definition vtow (v:Value) : Word := fst v.
+  Definition ztow (z:Z) : Word := ztow z.
+  Definition wtoz (w:Word) : Z := w.
+  
+  Definition Addr := Addr.
+  
+  Instance ShowWord : Show word :=
+    {| show x := show (word.signed x) |}.
+
+  Definition wlt := wlt.
+  Definition weq := weq.
+  Definition WordEqDec := WordEqDec.
+  Definition weq_implies_eq := weq_implies_eq.
+  Definition wle := wle.
+  Definition wplus := wplus.
+  Definition wminus := wminus.
+  Definition wplus_neq := wplus_neq.  
+  Definition Register := Register.
+  Definition RA := RA.
+  Definition SP := RA.
+  Definition regEqb := regEqb.
+  Definition callee_save := callee_save.
+  Definition RA_callee_save := RA_callee_save.
+  Definition SP_callee_save := SP_callee_save.
+
+  Inductive Element :=
+  | Mem (a:Addr)
+  | Reg (r:Register)
+  | PC.
+
+  Definition coercion1 (k:Element) :=
+    match k with
+    | Mem a => RISCV.Mem a
+    | Reg r => RISCV.Reg r
+    | PC => RISCV.PC
+    end.
+
+  Definition coercion2 (k:RISCV.Element) :=
+    match k with
+    | RISCV.Mem a => Mem a
+    | RISCV.Reg r => Reg r
+    | RISCV.PC => PC
+    end.
+  
+  Coercion coercion1 : Element >-> RISCV.Element.
+  Coercion coercion2 : RISCV.Element >-> Element.
+  
+  Definition keqb : Element -> Element -> bool := keqb.
+
+  Definition MachineState : Type := MPState.
+
+  Definition proj (m : MachineState) (k: Element) : Value :=
+    let '(m,p) := m in
+    (projw m k, projt p k).
+
+  Definition projw (m : MachineState) (k: Element): Word :=
+    let '(m,p) := m in
+    projw m k.
+  
+  Definition jorp (m : MachineState) (k : Element) (v : Value) : MachineState :=
+    let '(m,p) := m in
+    let '(w,t) := v in
+    let m' :=
+      match k with
+      | Mem a =>
+          withMem
+            (unchecked_store_byte_list (word.of_Z a)
+                                       (Z32s_to_bytes [w]) (getMem m)) m
+      | Reg r => 
+          withRegs (map.put (getRegs m) r (word.of_Z w)) m
+      | PC =>
+          withPc (word.of_Z w) m
+      end in
+    let p' := jorpt p k t in
+    (m',p').
+
+  Definition jorpw (m : MachineState) (k : Element) (w : Word) : MachineState :=
+    let '(m,p) := m in
+    let m' :=
+      match k with
+      | Mem a =>
+          withMem
+            (unchecked_store_byte_list (word.of_Z a)
+                                       (Z32s_to_bytes [w]) (getMem m)) m
+      | Reg r => 
+          withRegs (map.put (getRegs m) r (word.of_Z w)) m
+      | PC =>
+          withPc (word.of_Z w) m
+      end in
+    (m',p).
+  
+  Definition getElements (m : MachineState) : list Element :=
+    let '(m,p) := m in
+    map coercion2 (getElements m).
+
+  Definition Event := Event.
+  Definition event_eqb := event_eqb.
+    
+  Inductive Observation : Type := 
+  | Out (w:Event)
+  | Tau.
+
+  Definition coercion3 (obs:RISCV.Observation) :=
+    match obs with
+    | RISCV.Out w => Out w
+    | RISCV.Tau => Tau
+    end.
+  
+  Coercion coercion3 : RISCV.Observation >-> Observation.
+  
+  Definition obs_eqb (o1 o2 : Observation) : bool :=
+    match o1, o2 with
+    | Out e1, Out e2 => event_eqb e1 e2
+    | Tau, Tau => true
+    | _, _ => false
+    end.
+
+  (* Definition w32_eqb (w1 w2 : w32) : bool := *)
+  (*   let l1 := HList.tuple.to_list w1 in *)
+  (*   let l2 := HList.tuple.to_list w2 in *)
+  (*   let l12 := List.combine l1 l2 in *)
+  (*   forallb (fun '(b1, b2) => Byte.eqb b1 b2) l12. *)
+
+  (* Definition memAddr_eqb (mem mem' : DefaultMemImpl32.Mem) (addr : word32) : bool := *)
+  (*   match loadWord mem addr, loadWord mem' addr with *)
+  (*   | Some w, Some w' => w32_eqb w w' *)
+  (*   | _, _ => false *)
+  (*   end. *)
+
+  Definition listify1 {A} (m : Zkeyed_map A)
+    : list (Z * A) :=
+    List.rev (map.fold (fun acc z v => (z,v) :: acc) nil m).
+  
+  (* For now we will only monitor registers for changes. We could monitor
+     some memory, but we can't monitor the stack. *)
+  Definition findDiff (mOld mNew : MachineState) : option (Register*Word) :=
+    let '(mOld,pOld) := mOld in
+    let '(mNew,pNew) := mNew in
+    findDiff mOld mNew.
+
+  Definition FunID := nat.
+  Definition StackID := nat.
+
+  (* Definition EntryMap := Addr -> bool. *)
+
+  Definition StackMap := Addr -> option StackID.
+
+  (* Inductive CodeAnnotation := *)
+  (* | call *)
+  (* | retrn *)
+  (* | yield *)
+  (* | scall (f: MachineState -> Addr -> bool) *)
+  (* | normal *)
+  (* . *)
+  
+  (* Stack ID of stack pointer *)
+  Definition activeStack (sm: StackMap) (m: MachineState) :
+    option StackID :=
+    sm (projw m (Reg SP)).
+
+  Definition stack_eqb : StackID -> StackID -> bool :=
+    Nat.eqb.
+
+  Definition optstack_eqb (o1 o2 : option StackID) : bool :=
+    match o1, o2 with
+    | Some n1, Some n2 => stack_eqb n1 n2
+    | None, None => true
+    | _, _ => false
+    end.
+
+  (* Definition justRet (mc m: MachineState) : Prop := *)
+  (*   proj m PC = wplus (proj mc PC) 4 /\ proj m (Reg SP) = proj mc (Reg SP). *)
+
+  (* Definition justRet_dec mc m : {justRet mc m} + {~ justRet mc m}. *)
+  (* Proof. *)
+  (*   unfold justRet. *)
+  (*   destruct (WordEqDec (proj m PC) (wplus (proj mc PC) 4)); *)
+  (*     destruct (WordEqDec (proj m (Reg SP)) (proj mc (Reg SP))); *)
+  (*     try solve [left; auto]; *)
+  (*     right; intros [? ?]; auto. *)
+  (* Qed. *)
+
+  Inductive Operation : Type :=
+  | Call (f:FunID) (reg_args:list Register) (stk_args:list (Register*Z*Z))
+  | Tailcall (f:FunID) (reg_args:list Register) (stk_args:list (Register*Z*Z))
+  | Return
+  | Alloc (off:Z) (sz:Z)
+  | Dealloc (off:Z) (sz:Z)
+  .
+
+  Definition coercion4 (op : RISCV.Operation) :=
+    match op with
+    | RISCV.Call f reg_args stk_args => Call f reg_args stk_args
+    | RISCV.Tailcall f reg_args stk_args => Call f reg_args stk_args
+    | RISCV.Return => Return
+    | RISCV.Alloc off sz => Alloc off sz
+    | RISCV.Dealloc off sz => Dealloc off sz
+    end.
+
+  Coercion coercion4 : RISCV.Operation >-> Operation.
+  
+  Definition Operations := list Operation.
+
+  Definition CodeMap := Addr -> option Operations.
+  
+  (* TODO: operations *)
+  (* A Machine State can step to a new Machine State plus an Observation. *)
+  Definition step (m : MachineState) : MachineState * list Operation * Observation :=
+    let '(m',ops,obs) := mpstep m in
+    (m',map coercion4 ops, coercion3 obs).
+    
+End RISCVTagged.
